lean/5.lean
@@ -3,3 +3,4 @@ import «5».«5.1-parent-basic»
 import «5».«5.1-ancestor-basic»
 import «5».«5.1-ancestor-tree»
 import «5».«5.3-pred-is-oper1»
+import «5».«5.4-F-welldefined»
